src/lowparse/LowParse.Low.DER.fst
@@ -40,7 +40,7 @@ let validate_der_length_payload32
       if validator_max_length `U32.lt` v
       then v
       else
-        let z = read_u8 input pos in
+        let z = read_from_valid_slice read_u8 input pos in
         if z `U8.lt` 128uy
         then validator_error_generic
         else v
@@ -53,7 +53,7 @@ let validate_der_length_payload32
         if validator_max_length `U32.lt` v
         then v
         else
-          let y = read_bounded_integer_2 () input pos in
+          let y = read_from_valid_slice (read_bounded_integer_2 ()) input pos in
           if y `U32.lt `256ul
           then validator_error_generic
           else v
@@ -63,7 +63,7 @@ let validate_der_length_payload32
         if validator_max_length `U32.lt` v
         then v
         else
-          let y = read_bounded_integer_3 () input pos in
+          let y = read_from_valid_slice (read_bounded_integer_3 ()) input pos in
           if y `U32.lt `65536ul
           then validator_error_generic
           else v
@@ -72,7 +72,7 @@ let validate_der_length_payload32
         if validator_max_length `U32.lt` v
         then v
         else
-          let y = read_bounded_integer_4 () input pos in
+          let y = read_from_valid_slice (read_bounded_integer_4 ()) input pos in
           if y `U32.lt` 16777216ul
           then validator_error_generic
           else v
@@ -84,8 +84,8 @@ let jump_der_length_payload32
 = fun #rrel #rel input pos ->
     let h = HST.get () in
     [@inline_let] let _ =
-      valid_facts (parse_der_length_payload32 x) h input pos;
-      parse_der_length_payload32_unfold x (bytes_of_slice_from h input pos);
+      bvalid_facts (parse_der_length_payload32 x) h input pos;
+      parse_der_length_payload32_unfold x (bytes_of_buffer_from h input pos);
       assert_norm (pow2 (8 * 1) == 256);
       assert_norm (pow2 (8 * 2) == 65536);
       assert_norm (pow2 (8 * 3) == 16777216);
@@ -97,9 +97,9 @@ let jump_der_length_payload32
       [@inline_let]
       let len = x `U8.sub` 128uy in
       [@inline_let] let _ =
-        valid_facts parse_u8 h input pos;
+        bvalid_facts parse_u8 h input pos;
         parser_kind_prop_equiv parse_u8_kind parse_u8;
-        valid_facts (parse_bounded_integer (U8.v len)) h input pos;
+        bvalid_facts (parse_bounded_integer (U8.v len)) h input pos;
         parser_kind_prop_equiv (parse_bounded_integer_kind (U8.v len)) (parse_bounded_integer (U8.v len))
       in
       pos `U32.add` Cast.uint8_to_uint32 len
@@ -111,8 +111,8 @@ let read_der_length_payload32
 = fun #rrel #rel input pos ->
     let h = HST.get () in
     [@inline_let] let _ =
-      valid_facts (parse_der_length_payload32 x) h input pos;
-      parse_der_length_payload32_unfold x (bytes_of_slice_from h input pos);
+      bvalid_facts (parse_der_length_payload32 x) h input pos;
+      parse_der_length_payload32_unfold x (bytes_of_buffer_from h input pos);
       assert_norm (pow2 (8 * 1) == 256);
       assert_norm (pow2 (8 * 2) == 65536);
       assert_norm (pow2 (8 * 3) == 16777216);
@@ -126,14 +126,14 @@ let read_der_length_payload32
       (res <: refine_with_tag tag_of_der_length32 x)
     else if x = 129uy
     then
-      [@inline_let] let _ = valid_facts parse_u8 h input pos in
+      [@inline_let] let _ = bvalid_facts parse_u8 h input pos in
       let z = read_u8 input pos in
       [@inline_let] let res = Cast.uint8_to_uint32 z in
       [@inline_let] let _ = assert (tag_of_der_length32 res == x) in
       (res <: refine_with_tag tag_of_der_length32 x)
     else
       let len = x `U8.sub` 128uy in
-      [@inline_let] let _ = valid_facts (parse_bounded_integer (U8.v len)) h input pos in
+      [@inline_let] let _ = bvalid_facts (parse_bounded_integer (U8.v len)) h input pos in
       if len = 2uy
       then
         let res = read_bounded_integer_2 () input pos in
@@ -169,7 +169,7 @@ let validate_bounded_der_length32
     if validator_max_length `U32.lt` v
     then v
     else
-      let x = read_u8 input pos in
+      let x = read_from_valid_slice read_u8 input pos in
       let len = der_length_payload_size_of_tag8 x in
       let tg1 = tag_of_der_length32_impl min in
       let l1 = der_length_payload_size_of_tag8 tg1 in
@@ -183,7 +183,7 @@ let validate_bounded_der_length32
         if validator_max_length `U32.lt` v2
         then v2
         else
-          let y = read_der_length_payload32 x input v in
+          let y = read_from_valid_slice (read_der_length_payload32 x) input v in
           if y `U32.lt` min || max `U32.lt` y
           then validator_error_generic
           else v2
@@ -198,14 +198,14 @@ let jump_bounded_der_length32
     let h = HST.get () in
     [@inline_let]
     let _ =
-      valid_facts (parse_bounded_der_length32 (vmin) (vmax)) h input pos;
-      parse_bounded_der_length32_unfold (vmin) (vmax) (bytes_of_slice_from h input pos);
-      valid_facts parse_u8 h input pos
+      bvalid_facts (parse_bounded_der_length32 (vmin) (vmax)) h input pos;
+      parse_bounded_der_length32_unfold (vmin) (vmax) (bytes_of_buffer_from h input pos);
+      bvalid_facts parse_u8 h input pos
     in
     let v = jump_u8 input pos in
     let x = read_u8 input pos in
     let len = der_length_payload_size_of_tag8 x in
-    [@inline_let] let _ = valid_facts (parse_der_length_payload32 x) h input v in
+    [@inline_let] let _ = bvalid_facts (parse_der_length_payload32 x) h input v in
     jump_der_length_payload32 x input v
 
 inline_for_extraction
@@ -218,14 +218,14 @@ let read_bounded_der_length32
     let h = HST.get () in
     [@inline_let]
     let _ =
-      valid_facts (parse_bounded_der_length32 (vmin) (vmax)) h input pos;
-      parse_bounded_der_length32_unfold (vmin) (vmax) (bytes_of_slice_from h input pos);
-      valid_facts parse_u8 h input pos
+      bvalid_facts (parse_bounded_der_length32 (vmin) (vmax)) h input pos;
+      parse_bounded_der_length32_unfold (vmin) (vmax) (bytes_of_buffer_from h input pos);
+      bvalid_facts parse_u8 h input pos
     in
     let v = jump_u8 input pos in
     let x = read_u8 input pos in
     let len = der_length_payload_size_of_tag8 x in
-    [@inline_let] let _ = valid_facts (parse_der_length_payload32 x) h input v in
+    [@inline_let] let _ = bvalid_facts (parse_der_length_payload32 x) h input v in
     let y = read_der_length_payload32 x input v in
     (y <: bounded_int32 (vmin) (vmax))
 
